ironfleet/src/Dafny/Distributed/Impl/Raft/CTypes.i.dfy
@@ -1,0 +1,19 @@
+include "../../Services/Raft/AppStateMachine.s.dfy"
+include "../../Common/Framework/Environment.s.dfy"
+include "../../Common/Native/Io.s.dfy"
+include "AppInterface.i.dfy"
+
+module Raft__CTypes_i {
+
+import opened Raft__AppInterface_i
+import opened AppStateMachine_s
+import opened Environment_s
+import opened Native__Io_s
+
+datatype CLogEntry = CLogEntry(term:uint64, index:uint64, req:CAppRequest, is_commited:bool)
+
+predicate CLogEntryValid(entry:CLogEntry) {
+  && entry.term > 0 && entry.index > 0
+}
+
+}
