ironfleet/src/Dafny/Distributed/Impl/Raft/Config.i.dfy
@@ -1,0 +1,83 @@
+include "../../Common/Native/Io.s.dfy"
+include "../../Common/Collections/Sets.i.dfy"
+include "../../Common/Collections/Seqs.i.dfy"
+include "../../Common/Collections/Maps2.s.dfy"
+include "../../Common/Native/NativeTypes.s.dfy"
+include "../Common/UpperBound.i.dfy"
+include "../../Protocol/Raft/Config.i.dfy"
+
+module Raft__ConfigState_i {
+
+import opened Common__UpperBound_s
+import opened Native__Io_s
+import opened Native__NativeTypes_s
+import opened Collections__Sets_i
+import opened Collections__Seqs_i
+import opened Collections__Maps2_s
+import opened Raft__Config_i
+
+datatype ParamState = ParamState(
+  min_election_timeout:uint64,
+  max_election_timeout:uint64,
+  heartbeat_timeout:uint64,
+  max_integer_value:uint64
+)
+
+function AbstractifyParamStateToRaftParam(params:ParamState) : RaftParam
+{
+  RaftParam(
+    params.min_election_timeout as int,
+    params.max_election_timeout as int,
+    params.heartbeat_timeout as int,
+    UpperBoundFinite(params.max_integer_value as int)
+  )       
+}
+
+function method StaticParams():ParamState
+{
+  ParamState(
+    1000, // min_election_timeout
+    2000, // max_election_timeout
+    100, // heartbeat_timeout
+    0x8000_0000_0000_0000 - 1 // max_integer_value
+  )
+}
+
+datatype ConfigState = ConfigState(
+  // client_eps:set<EndPoint>,
+  server_eps:seq<EndPoint>,
+  params:ParamState
+)
+
+function AbstractifyConfigStateToRaftConfig(config:ConfigState) : RaftConfig
+{
+  RaftConfig(
+    config.server_eps,
+    AbstractifyParamStateToRaftParam(config.params)
+  )
+}
+
+datatype ServerConfigState = ServerConfigState(
+  server_ep:EndPoint,
+  global_config:ConfigState
+)
+
+function AbstractifyServerConfigStateToRaftServerConfig(server_config:ServerConfigState) : RaftServerConfig
+{
+  RaftServerConfig(
+    server_config.server_ep,
+    AbstractifyConfigStateToRaftConfig(server_config.global_config)
+  )
+}
+
+method InitServerConfigState(my_ep:EndPoint, eps:seq<EndPoint>) returns (sc:ServerConfigState)
+  ensures sc.server_ep == my_ep
+  ensures sc.global_config.server_eps == eps
+  ensures sc.global_config.params == StaticParams()
+{
+  var params := StaticParams(); 
+  var global_config := ConfigState(eps, params);
+  sc := ServerConfigState(my_ep, global_config);
+}
+
+}
