ironfleet/src/Dafny/Distributed/Impl/Raft/Host.i.dfy
@@ -1,0 +1,100 @@
+include "CmdLineParser.i.dfy"
+include "Config.i.dfy"
+include "ServerImpl.i.dfy"
+include "../../Common/Framework/Host.s.dfy"
+include "../../Common/Collections/Sets.i.dfy"
+include "../../Protocol/Raft/ServerScheduler.i.dfy"
+
+module Host_i refines Host_s {
+import opened RaftCmdLineParser_i
+import opened Raft__ConfigState_i
+import opened Collections__Sets_i
+import opened Raft__ServerScheduler_i
+import opened Raft__ServerImpl_i
+export Spec
+    provides Native__Io_s, Environment_s, Native__NativeTypes_s
+    provides HostState
+    provides ConcreteConfiguration
+    provides HostInit, HostNext, ConcreteConfigInit, HostStateInvariants
+    provides ConcreteConfigToServers, ParseCommandLineConfiguration, ArbitraryObject
+    provides HostInitImpl, HostNextImpl
+export All reveals *
+
+datatype CScheduler = CScheduler(ghost sched:RaftServerScheduler, server_impl:ServerImpl)
+
+type HostState = CScheduler
+type ConcreteConfiguration = ConfigState
+
+predicate HostInit(host_state:HostState, config:ConcreteConfiguration, id:EndPoint)
+{
+  id in config.server_eps
+}
+predicate HostNext(host_state:HostState, host_state':HostState, ios:seq<LIoOp<EndPoint, seq<byte>>>)
+{
+  && host_state' == host_state
+  && |ios| == 0
+}
+
+predicate ConcreteConfigInit(config:ConcreteConfiguration)
+{
+  true
+}
+
+predicate HostStateInvariants(host_state:HostState, env:HostEnvironment)
+{
+  true
+}
+
+function ConcreteConfigToServers(config:ConcreteConfiguration) : set<EndPoint>
+{
+  MapSeqToSet(config.server_eps, x=>x)
+}
+
+function ParseCommandLineConfiguration(args:seq<seq<byte>>) : ConcreteConfiguration
+{
+  var server_eps := raft_config_parsing(args);
+  var config := ConfigState(
+    server_eps, // server_eps
+    StaticParams()
+  );
+  config
+}
+
+method {:timeLimitMultiplier 4} HostInitImpl(ghost env:HostEnvironment, netc:NetClient, args:seq<seq<byte>>) returns (
+    ok:bool,
+    host_state:HostState
+)
+{
+  var my_index;
+  var server_eps;
+  var raft_sched:RaftServerScheduler;
+  var server := new ServerImpl();
+  host_state := CScheduler(raft_sched, server);
+
+  var ep := EndPoint(netc.MyPublicKey());
+  ok, server_eps, my_index := parse_cmd_line(ep, args);
+  if !ok { return; }
+  print "My ep is: ", ep, "\n";
+
+  var server_config := InitServerConfigState(ep, server_eps);
+  host_state := CScheduler(server.AbstractifyToRaftServerScheduler(), server);
+}
+
+method HostNextImpl(ghost env:HostEnvironment, host_state:HostState) 
+  returns (
+  ok:bool,
+  host_state':HostState,
+  ghost recvs:seq<NetEvent>,
+  ghost clocks:seq<NetEvent>,
+  ghost sends:seq<NetEvent>,
+  ghost ios:seq<LIoOp<EndPoint, seq<byte>>>
+)
+{
+  ok := true;
+  host_state' := host_state;
+  recvs := [];
+  clocks := [];
+  sends := [];
+  ios := [];
+}
+}
