ironfleet/src/Dafny/Distributed/Impl/Raft/PacketParsing.i.dfy
@@ -1,0 +1,225 @@
+include "../../Common/Collections/Maps.i.dfy"
+include "../../Protocol/Raft/Types.i.dfy"
+include "../Common/GenericMarshalling.i.dfy"
+include "CTypes.i.dfy"
+
+module Raft__PacketParsing_i {
+
+import opened Native__Io_s
+import opened Native__NativeTypes_s
+import opened Collections__Maps_i
+import opened Raft__AppInterface_i
+import opened Raft__Types_i
+import opened Raft__CTypes_i
+import opened Common__GenericMarshalling_i
+import opened Common__NodeIdentity_i
+import opened Common__NetClient_i
+import opened Common__Util_i
+import opened AppStateMachine_s
+import opened Environment_s
+import opened Math__mul_i
+import opened Math__mul_nonlinear_i
+
+////////////////////////////////////////////////////////////////////
+//    Grammars for the Rafy types
+////////////////////////////////////////////////////////////////////
+function method EndPoint_grammar() : G { GByteArray }
+function method CLogEntry_grammar() : G { GTuple([GUint64, GUint64, GByteArray, GUint64]) }
+function method CLogEntrySeq_grammar() : G { GArray(CLogEntry_grammar()) }
+
+////////////////////////////////////////////////////////////////////
+//    Grammars for the Raft messages 
+////////////////////////////////////////////////////////////////////
+function method CMessage_RequestVote_grammar() : G { GTuple([GUint64, EndPoint_grammar(), GUint64, GUint64]) }
+function method CMessage_RequestVoteReply_grammar() : G { GTuple([GUint64, GUint64]) }
+function method CMessage_AppendEntries_grammar() : G { GTuple([GUint64, EndPoint_grammar(), GUint64, GUint64, CLogEntrySeq_grammar(), GUint64]) }
+function method CMessage_AppendEntriesReply_grammar() : G { GTuple([GUint64, GUint64, GUint64]) }
+
+function method CMessage_grammar() : G { 
+  GTaggedUnion([
+    CMessage_RequestVote_grammar(),
+    CMessage_RequestVoteReply_grammar(),
+    CMessage_AppendEntries_grammar(),
+    CMessage_AppendEntriesReply_grammar()
+  ]) 
+}
+
+predicate NetPacketBound(data:seq<byte>) 
+{
+  |data| < MaxPacketSize()
+}
+
+predicate CMessageIs64Bit(msg:CMessage)
+{
+  true
+}
+
+
+////////////////////////////////////////////////////////////////////
+//    Parsing
+////////////////////////////////////////////////////////////////////
+function method parse_EndPoint(val:V) : EndPoint
+  requires ValInGrammar(val, EndPoint_grammar())
+  ensures  EndPointIsAbstractable(parse_EndPoint(val))
+{
+  EndPoint(val.b)
+}
+
+function method parse_CLogEntry(val:V) : CLogEntry
+  requires ValInGrammar(val, CLogEntry_grammar())
+  ensures  CLogEntryIsAbstractable(parse_CLogEntry(val))
+{
+  CLogEntry(val.t[0].u, val.t[1].u, val.t[2].b, val.t[3].u)
+}
+
+function method parse_Message_RequestVote(val:V) : CMessage
+  requires ValInGrammar(val, CMessage_RequestVote_grammar())
+  ensures CMesssageIsAbstractable(parse_Message_RequestVote(val))
+  ensures  ValidVal(val) ==> CMessageIs64Bit(parse_Message_RequestVote(val))
+{
+  CMessage_RequestVote(
+    val.t[0].u,
+    parse_EndPoint(val.t[1]),
+    val.t[2].u,
+    val.t[3].u
+  )
+}
+
+function method parse_Message_RequestVoteReply(val:V) : CMessage
+  requires ValInGrammar(val, CMessage_RequestVoteReply_grammar())
+  ensures CMesssageIsAbstractable(parse_Message_RequestVoteReply(val))
+  ensures  ValidVal(val) ==> CMessageIs64Bit(parse_Message_RequestVoteReply(val))
+{
+  CMessage_RequestVoteReply(
+    val.t[0].u,
+    val.t[1].u
+  )
+}
+
+function parse_CLogEntrySeq(val:V) : seq<CLogEntry>
+  requires ValInGrammar(val, CLogEntrySeq())
+  ensures  |parse_CLogEntrySeq(val)| == |val.a|
+  ensures  forall i :: 0 <= i < |parse_CLogEntrySeq(val)| ==> parse_CLogEntrySeq(val)[i] == parse_CLogEntry(val.a[i])
+  ensures  CRequestBatchIsAbstractable(parse_CLogEntrySeq(val))
+  ensures  ValidVal(val) ==> CRequestBatchIs64Bit(parse_CLogEntrySeq(val))
+  decreases |val.a|
+{
+  if |val.a| == 0 then
+    []
+  else 
+    var req := parse_CLogEntry(val.a[0]);
+    var restVal:V := VArray(val.a[1..]);
+    var rest := parse_CLogEntrySeq(restVal);
+    [req] + rest
+}
+
+function method parse_Message_AppendEntries(val:V) : CMessage
+  requires ValInGrammar(val, CMessage_AppendEntries_grammar())
+  ensures CMesssageIsAbstractable(parse_Message_AppendEntries(val))
+  ensures  ValidVal(val) ==> CMessageIs64Bit(parse_Message_AppendEntries(val))
+{
+  CMessage_AppendEntries(
+    val.t[0].u,
+    parse_EndPoint(val.t[1]),
+    val.t[2].u,
+    val.t[3].u,
+    parse_CLogEntrySeq(val.t[4]),
+    val.t[5].u
+  )
+}
+
+function method parse_Message_AppendEntriesReply(val:V) : CMessage
+  requires ValInGrammar(val, CMessage_AppendEntriesReply_grammar())
+  ensures CMesssageIsAbstractable(parse_Message_AppendEntriesReply(val))
+  ensures  ValidVal(val) ==> CMessageIs64Bit(parse_Message_AppendEntriesReply(val))
+{
+  CMessage_AppendEntriesReply(
+    val.t[0].u,
+    val.t[1].u,
+    val.t[2].u
+  )
+}
+
+method Parse_Message(val:V) returns (msg:CMessage)
+	requires ValInGrammar(val, CMessage_grammar())
+	requires ValidVal(val)
+	// ensures	 msg == parse_Message(val)
+	ensures	 !msg.CMessage_Invalid?
+	ensures	 CMessageIsAbstractable(msg)
+	ensures	 CMessageIs64Bit(msg)
+{
+  if val.c == 0 {
+    msg := parse_Message_RequestVote(val.val);
+  } else if val.c == 1 {
+    msg := parse_Message_RequestVoteReply(val.val);
+  } else if val.c == 2 {
+    msg := parse_Message_AppendEntries(val.val);
+  } else if val.c == 3 {
+    msg := parse_Message_AppendEntriesReply(val.val);
+  } else {
+    assert false;
+  }
+}
+
+
+////////////////////////////////////////////////////////////////////
+//    Demarshall
+////////////////////////////////////////////////////////////////////
+function RaftDemarshallData(data:seq<byte>) : CMessage
+  ensures  CMessageIsAbstractable(RaftDemarshallData(data))
+{
+  if Demarshallable(data, CMessage_grammar()) then
+    var val := DemarshallFunc(data, CMessage_grammar());
+    parse_Message(val)
+  else
+    CMessage_Invalid()
+}
+
+method RaftDemarshallDataMethod(data:array<byte>, msg_grammar:G) returns (msg:CMessage)
+  requires data.Length < 0x1_0000_0000_0000_0000
+  requires msg_grammar == CMessage_grammar()
+  requires ValidGrammar(msg_grammar)
+  ensures  CMessageIsAbstractable(msg)
+  ensures  if Demarshallable(data[..], msg_grammar) then
+             msg == RaftDemarshallData(data[..]) 
+           else
+             msg.CMessage_Invalid?
+  ensures  CMessageIs64Bit(msg)
+{
+  var success, val := Demarshall(data, msg_grammar);
+  if success {
+    assert ValInGrammar(val, msg_grammar);
+    msg := Parse_Message(val);
+    assert !msg.CMessage_Invalid?;
+  } else {
+    msg := CMessage_Invalid();
+  }
+}
+
+////////////////////////////////////////////////////////////////////
+//    Can a value be marshalled?
+////////////////////////////////////////////////////////////////////
+function Marshallable(msg:CMessage) : bool
+{
+  // TODO: this is a hack
+  && (!msg.CMessage_Invalid?)
+  && (msg.CMessage_RequestVote? ==> true)
+  && (msg.CMessage_RequestVoteReply? ==> true)
+  && (msg.CMessage_AppendEntries? ==> true)
+  && (msg.CMessage_AppendEntriesReply? ==> true)
+}
+
+function CMessageIsValid(msg:CMessage) : bool
+{
+  Marshallable(msg)
+}
+
+predicate CPacketsIsMarshallable(cps:set<CPacket>)
+{
+  forall cp :: cp in cps ==> Marshallable(cp.msg)
+}
+
+// TODO & DOING: finish this about determining if valid and DetermineIfMessageMarshallable
+
+
+}
