ironfleet/src/Dafny/Distributed/Impl/Raft/ServerImpl.i.dfy
@@ -1,0 +1,122 @@
+include "../../Common/Framework/Environment.s.dfy"
+include "../../Common/Logic/Option.i.dfy"
+include "../../Common/Native/NativeTypes.s.dfy"
+include "../../Common/Native/Io.s.dfy"
+include "../../Protocol/Raft/Config.i.dfy"
+include "../../Protocol/Raft/Server.i.dfy"
+include "../../Protocol/Raft/ServerScheduler.i.dfy"
+include "../../Protocol/Raft/Types.i.dfy"
+include "../../Services/Raft/AppStateMachine.s.dfy"
+include "../Common/GenericMarshalling.i.dfy"
+include "../Common/NetClient.i.dfy"
+include "Config.i.dfy"
+
+module Raft__ServerImpl_i {
+
+import opened Logic__Option_i
+import opened Native__Io_s
+import opened Native__NativeTypes_s
+import opened Raft__Config_i
+import opened Raft__Server_i
+import opened Raft__ServerScheduler_i
+import opened Raft__Types_i
+import opened Common__GenericMarshalling_i
+import opened Common__NetClient_i
+import opened AppStateMachine_s
+import opened Raft__ConfigState_i
+
+class ServerImpl
+{
+  var net_client:NetClient?;
+  var local_addr:EndPoint;
+  var nextActionIndex:uint64;
+
+  var config:ServerConfigState;
+  var role:RaftRole;
+  // for timeout
+  var next_heartbeat_time:uint64;
+  var next_election_time:uint64;
+  // persistent state
+  var current_leader:Option<EndPoint>;
+  var current_term:uint64;
+  var voted_for:Option<EndPoint>;
+  var log:seq<LogEntry>;
+  // volatile state on all servers
+  var commit_index:uint64;
+  var last_applied:uint64;
+  // volatile state on leaders
+  var next_index:map<EndPoint, int>;
+  var match_index:map<EndPoint, int>;
+  var num_replicated:seq<int>; // log index -> num of replicated
+
+  var msg_grammar:G;
+
+  var app_state:AppStateMachine;
+
+  constructor() {
+    net_client := null;
+    role := Follower;
+    next_heartbeat_time := 0;
+    next_election_time := 0;
+    current_leader := None();
+    current_term := 0;
+    voted_for := None();
+    log := [];
+    commit_index := 0;
+    last_applied := 0;
+    next_index := map[];
+    match_index := map[];
+    num_replicated := [];
+    msg_grammar := 
+    var app_s := AppStateMachine.Initialize();
+    app_state := app_s;
+  }
+
+  function AbstractifyToRaftServer() : RaftServer
+    reads this
+  {
+    RaftServer(
+      AbstractifyServerConfigStateToRaftServerConfig(config),
+      role,
+      next_heartbeat_time as int,
+      next_election_time as int,
+      current_leader,
+      current_term as int,
+      voted_for,
+      log,
+      commit_index as int,
+      last_applied as int,
+      next_index,
+      match_index,
+      num_replicated,
+      app_state.Abstractify()
+    )
+  }
+
+  function AbstractifyToRaftServerScheduler() : RaftServerScheduler
+    reads this
+  {
+    RaftServerScheduler(
+      this.AbstractifyToRaftServer(),
+      this.nextActionIndex as int
+    )
+  }
+
+  method Init(
+    config:ServerConfigState,
+    nc:NetClient,
+    ghost env:HostEnvironment
+  ) returns (ok:bool)
+    requires env.Valid() && env.ok.ok()
+    requires NetClientIsValid(nc)
+    requires WellFormedRaftServerConfig(AbstractifyServerConfigStateToRaftServerConfig(config))
+    modifies this
+  {
+    this.config := config;
+    this.net_client := nc;
+    this.nextActionIndex := 0;
+    this.msg_grammar := CMessage_grammar();
+    ok := true;
+  }
+}
+}
